Initial review of Materials.dfy (#160)
* Review Materials.dfy

- Remove `method` keyword from functions where able.
- Add EncryptionContextGet() to replace EncCtxLookup (EncCtxLookup is
now a ghost function backing EncryptionContextGet).
- Add FunctionFind(), like Find(), but works with a T -> bool lambda.
- Removed unused methods.
- Add tests

* Remove "UTF8" from test names.

* Add EncryptionContextGet test covering very large EncryptionContexts

* Rename Find functions

* Mitigating Base64 timeouts

- Add ensures to Base64.Encode()
- Add lemma ensuring validity of BASE64_TEST_VECTORS_ENCODED

* Fixing previously uncaught merge conflicts

src/SDK/Materials.dfy
@@ -9,10 +9,43 @@ module {:extern "Materials"} Materials {
   import UTF8
   import AlgorithmSuite
 
+  // TODO: Update EncryptionContext structure to a map structure.
+  // https://github.com/awslabs/aws-encryption-sdk-dafny/issues/50
   type EncryptionContext = seq<(UTF8.ValidUTF8Bytes, UTF8.ValidUTF8Bytes)>
 
   function method GetKeysFromEncryptionContext(encryptionContext: EncryptionContext): set<UTF8.ValidUTF8Bytes> {
     set i | 0 <= i < |encryptionContext| :: encryptionContext[i].0
+  }
+
+  method EncryptionContextGet(encryptionContext: EncryptionContext, key: UTF8.ValidUTF8Bytes) returns (res: Result<UTF8.ValidUTF8Bytes>)
+    ensures match EncCtxLookup(encryptionContext, key)
+            case Some(value) => res.Success? && res.value == value
+            case None => res.Failure? && res.error == "Key not found."
+  {
+    res := Failure("Key not found.");
+    var i := 0;
+    while i < |encryptionContext|
+      invariant i <= |encryptionContext|
+      invariant forall j :: 0 <= j < i ==> encryptionContext[j].0 != key
+    {
+      if encryptionContext[i].0 == key {
+        res := Success(encryptionContext[i].1);
+        return res;
+      }
+      i := i + 1;
+    }
+  }
+
+  function EncCtxLookup(x: EncryptionContext, k: UTF8.ValidUTF8Bytes): Option<UTF8.ValidUTF8Bytes>
+  {
+    match EncCtxIndexLookup(x, k)
+    case Some(i) => Some(x[i].1)
+    case None => None
+  }
+
+  function EncCtxIndexLookup(x: EncryptionContext, k: UTF8.ValidUTF8Bytes): (opt: Option<nat>)
+  {
+    FindIndex(x, (y: (UTF8.ValidUTF8Bytes, UTF8.ValidUTF8Bytes)) => y.0 == k, 0)
   }
 
   // UTF-8 encoded "aws-crypto-public-key"
@@ -69,7 +102,7 @@ module {:extern "Materials"} Materials {
                                                encryptedDataKeys: seq<ValidEncryptedDataKey>,
                                                keyringTrace: seq<KeyringTraceEntry>)
   {
-    predicate method Valid() {
+    predicate Valid() {
       var generateTraces := Filter(keyringTrace, IsGenerateTraceEntry);
       var encryptTraces := Filter(keyringTrace, IsEncryptTraceEntry);
       && algorithmSuiteID.ValidPlaintextDataKey(plaintextDataKey)
@@ -135,7 +168,7 @@ module {:extern "Materials"} Materials {
                                                      dataKeyMaterials: ValidDataKeyMaterials,
                                                      signingKey: Option<seq<uint8>>)
   {
-    predicate method Valid() {
+    predicate Valid() {
       && dataKeyMaterials.algorithmSuiteID.SignatureType().Some? ==> signingKey.Some?
       && |dataKeyMaterials.encryptedDataKeys| > 0
     }
@@ -154,7 +187,7 @@ module {:extern "Materials"} Materials {
                                                      keyringTrace: seq<KeyringTraceEntry>)
 
   {
-    predicate method Valid() {
+    predicate Valid() {
       && algorithmSuiteID.ValidPlaintextDataKey(plaintextDataKey)
       && algorithmSuiteID.SignatureType().Some? ==> verificationKey.Some?
       && (forall entry :: entry in keyringTrace ==> entry.flags <= ValidDecryptionMaterialFlags)
@@ -168,59 +201,4 @@ module {:extern "Materials"} Materials {
   }
 
   type ValidDecryptionMaterials = i: DecryptionMaterials | i.Valid() witness DecryptionMaterials.ValidWitness()
-
-    //TODO: Review this code.
-    function method naive_merge<T> (x : seq<T>, y : seq<T>, lt : (T, T) -> bool) : seq<T>
-    {
-        if |x| == 0 then y
-        else if |y| == 0 then x
-        else if lt(x[0], y[0]) then [x[0]] + naive_merge(x[1..], y, lt)
-        else [y[0]] + naive_merge(x, y[1..], lt)
-    }
-
-    function method naive_merge_sort<T> (x : seq<T>, lt : (T, T) -> bool) : seq<T>
-    {
-        if |x| < 2 then x else
-        var t := |x| / 2; naive_merge(naive_merge_sort(x[..t], lt), naive_merge_sort(x[t..], lt), lt)
-
-    }
-
-    function method memcmp_le (a : seq<uint8>, b : seq<uint8>, len : nat) : (res : Option<bool>)
-        requires |a| >= len
-        requires |b| >= len {
-        if len == 0 then None else if a[0] != b[0] then Some(a[0] < b[0]) else memcmp_le (a[1..], b[1..], len - 1)
-    }
-
-    predicate method lex_lt(b : seq<uint8>, a : seq<uint8>)
-    {
-        match memcmp_le(a,b, if |a| < |b| then |a| else |b|) {
-        case Some(b) => !b
-        case None => !(|a| <= |b|)
-        }
-    }
-
-    predicate method lt_keys(b : (seq<uint8>, seq<uint8>), a : (seq<uint8>, seq<uint8>)) {
-        lex_lt(b.0, a.0)
-    }
-
-    function method EncCtxFlatten (x : seq<(UTF8.ValidUTF8Bytes, UTF8.ValidUTF8Bytes)>): UTF8.ValidUTF8Bytes {
-        if x == [] then [] else
-        x[0].0 + x[0].1 + EncCtxFlatten(x[1..])
-    }
-
-    function method FlattenSortEncCtx(x : seq<(UTF8.ValidUTF8Bytes, UTF8.ValidUTF8Bytes)>): UTF8.ValidUTF8Bytes
-    {
-        EncCtxFlatten(naive_merge_sort(x, lt_keys))
-    }
-
-    function method EncCtxLookup(x : seq<(UTF8.ValidUTF8Bytes, UTF8.ValidUTF8Bytes)>, k : UTF8.ValidUTF8Bytes): Option<UTF8.ValidUTF8Bytes>
-    {
-        if |x| == 0 then None else
-        if x[0].0 == k then Some(x[0].1) else EncCtxLookup(x[1..], k)
-    }
-
-    function method EncCtxOfStrings(x : seq<(UTF8.ValidUTF8Bytes, UTF8.ValidUTF8Bytes)>): seq<(UTF8.ValidUTF8Bytes, UTF8.ValidUTF8Bytes)>  {
-        if x == [] then [] else
-        [(x[0].0, x[0].1)] + EncCtxOfStrings(x[1..])
-    }
 }
